utils.v
@@ -4,16 +4,13 @@ Require Import Coq.Lists.List.
 Import ListNotations.
 
 Module Utils.
+
   (* TODO: Use N as fuel with {measure N.to_nat fuel} *)
-  Function run {State: Type} (step: State -> option State)
-           (state: State) (output: State -> list nat)
-           (fuel: nat): option (list nat) :=
+  Function run {State: Type} (step: State -> State)
+           (state: State) (fuel: nat): State :=
     match fuel with
-    | 0 => None
-    | S f =>
-      match step state with
-      | None => Some (output state)
-      | Some state' => run step state' output f
-      end
+    | 0 => state
+    | S f => run step (step state) f
     end.
+
 End Utils.
